compiler/backend/ag32/proofs/ag32_ffi_codeProofScript.sml
@@ -27,7 +27,11 @@ fun next_tac n =
     \\ qmatch_goalsub_abbrev_tac`pc + 2w`
     \\ simp[GSYM get_mem_word_def]
     \\ `^sn.PC = s.PC + n2w(4 * ^(numSyntax.term_of_int n))`
-    by ( simp[Abbr`^sn`, dfn'Normal_PC] )
+    by ( simp[Abbr`^sn`,
+              dfn'Normal_PC,
+              dfn'LoadMEMByte_PC,
+              dfn'Shift_PC,
+              dfn'LoadConstant_PC] )
     \\ `byte_aligned ^sn.PC`
     by (
       simp[]
@@ -37,10 +41,21 @@ fun next_tac n =
     \\ simp[]
     \\ disch_then kall_tac
     \\ qpat_x_assum`Abbrev(pc = _)`kall_tac
-    \\ first_assum(qspec_then`^(numSyntax.term_of_int n)`mp_tac)
+    \\ last_assum(qspec_then`^(numSyntax.term_of_int n)`mp_tac)
     \\ impl_tac >- EVAL_TAC
-    \\ simp_tac(srw_ss())[ag32_ffi_return_code_def]
-    \\ `^sn.MEM = s.MEM` by simp[Abbr`^sn`,dfn'Normal_MEM]
+    \\ simp_tac(srw_ss())[ag32_ffi_write_check_conf_code_def,
+                          ag32_ffi_write_load_noff_code_def,
+                          ag32_ffi_write_check_lengths_code_def,
+                          ag32_ffi_write_write_header_code_def,
+                          ag32_ffi_write_num_written_code_def,
+                          ag32_ffi_copy_code_def,
+                          ag32_ffi_return_code_def]
+    \\ `^sn.MEM = s.MEM`
+    by simp[Abbr`^sn`,
+            dfn'Normal_MEM,
+            dfn'LoadMEMByte_MEM,
+            dfn'Shift_MEM,
+            dfn'LoadConstant_MEM]
     \\ simp[]
     \\ disch_then kall_tac
     \\ simp[ag32_targetProofTheory.Decode_Encode]
@@ -92,6 +107,229 @@ val ag32_ffi_return_code_thm = Q.store_thm("ag32_ffi_return_code_thm",
   \\ simp[ag32_targetProofTheory.Decode_Encode]
   \\ simp[ag32Theory.Run_def]
   \\ simp[Once EXISTS_NUM]);
+
+val ag32_ffi_copy_code_thm = Q.store_thm("ag32_ffi_copy_code_thm",
+  `∀s.
+   (∀k. k < LENGTH ag32_ffi_copy_code ⇒
+        (get_mem_word s.MEM (s.PC + n2w (4 * k)) =
+         Encode (EL k ag32_ffi_copy_code)))
+   ∧ byte_aligned s.PC
+   ∧ w2n s.PC + 4 * LENGTH ag32_ffi_copy_code < dimword (:32)
+   ∧ w2n (s.R 5w) + w2n (s.R 1w) < dimword(:32)
+   ∧ DISJOINT { s.R 5w + n2w k | k | k < w2n (s.R 1w) }
+              { s.PC + n2w k | k | k DIV 4 < LENGTH ag32_ffi_copy_code }
+   ⇒
+   ∃k. (FUNPOW Next k s = ag32_ffi_copy s)`,
+  Induct_on`w2n(s.R 1w)` \\ rw[]
+  >- (
+    simp[Once ag32_ffi_copy_def]
+    \\ Cases_on`s.R 1w` \\ fs[] \\ rw[]
+    \\ qexists_tac`1` \\ rw[]
+    \\ rw[ag32Theory.Next_def]
+    \\ qmatch_goalsub_abbrev_tac`pc + 2w`
+    \\ simp[GSYM get_mem_word_def]
+    \\ last_assum(qspec_then`0`mp_tac)
+    \\ impl_tac >- EVAL_TAC
+    \\ simp_tac(srw_ss())[]
+    \\ pop_assum mp_tac
+    \\ DEP_REWRITE_TAC[byte_aligned_imp]
+    \\ conj_tac >- rw[]
+    \\ strip_tac \\ simp[Abbr`pc`]
+    \\ disch_then kall_tac
+    \\ simp[ag32_ffi_copy_code_def]
+    \\ simp[ag32_targetProofTheory.Decode_Encode]
+    \\ simp[ag32Theory.Run_def] )
+  \\ simp[Once ag32_ffi_copy_def]
+  \\ Cases_on`s.R 1w` \\ fs[]
+  \\ simp[Once EXISTS_NUM] \\ disj2_tac \\ simp[FUNPOW]
+  \\ simp[ag32Theory.Next_def]
+  \\ qmatch_goalsub_abbrev_tac`pc + 2w`
+  \\ simp[GSYM get_mem_word_def]
+  \\ qpat_x_assum`Abbrev(pc = _)`mp_tac
+  \\ DEP_REWRITE_TAC[byte_aligned_imp]
+  \\ conj_tac
+  >- ( simp[] \\ irule byte_aligned_add \\ fs[] \\ EVAL_TAC )
+  \\ strip_tac \\ fs[Abbr`pc`]
+  \\ first_assum(qspec_then`0`mp_tac)
+  \\ impl_tac >- EVAL_TAC
+  \\ simp[]
+  \\ simp[ag32_targetProofTheory.Decode_Encode]
+  \\ simp[ag32_ffi_copy_code_def]
+  \\ disch_then kall_tac
+  \\ simp[ag32Theory.Run_def]
+  \\ simp[Once EXISTS_NUM] \\ disj2_tac \\ simp[FUNPOW]
+  \\ qmatch_goalsub_abbrev_tac`Next s1`
+  \\ simp[ag32Theory.Next_def]
+  \\ qmatch_goalsub_abbrev_tac`pc + 2w`
+  \\ simp[GSYM get_mem_word_def]
+  \\ `s1.PC = s.PC + n2w (4 * 1)`
+  by ( simp[Abbr`s1`, ag32Theory.dfn'JumpIfZero_def, ag32Theory.ri2word_def,
+            ag32Theory.ALU_def,ag32Theory.incPC_def] )
+  \\ qpat_x_assum`Abbrev(pc = _)`mp_tac
+  \\ DEP_REWRITE_TAC[byte_aligned_imp]
+  \\ conj_tac
+  >- ( simp[] \\ irule byte_aligned_add \\ fs[] \\ EVAL_TAC )
+  \\ strip_tac \\ fs[Abbr`pc`]
+  \\ `s1.MEM = s.MEM` by simp[Abbr`s1`, dfn'JumpIfZero_MEM]
+  \\ first_assum(qspec_then`1`mp_tac)
+  \\ impl_tac >- EVAL_TAC
+  \\ simp[]
+  \\ simp[ag32_targetProofTheory.Decode_Encode]
+  \\ simp[ag32_ffi_copy_code_def]
+  \\ disch_then kall_tac
+  \\ simp[ag32Theory.Run_def]
+  \\ next_tac 2
+  \\ simp[Once EXISTS_NUM] \\ disj2_tac \\ simp[FUNPOW]
+  \\ qmatch_goalsub_abbrev_tac`Next s3`
+  \\ simp[ag32Theory.Next_def]
+  \\ qmatch_goalsub_abbrev_tac`pc + 2w`
+  \\ simp[GSYM get_mem_word_def]
+  \\ `s3.PC = s.PC + n2w (4 * 3)`
+  by ( simp[Abbr`s3`, ag32Theory.dfn'StoreMEMByte_def, ag32Theory.incPC_def] )
+  \\ qpat_x_assum`Abbrev(pc = _)`mp_tac
+  \\ DEP_REWRITE_TAC[byte_aligned_imp]
+  \\ conj_tac
+  >- ( simp[] \\ irule byte_aligned_add \\ fs[] \\ EVAL_TAC )
+  \\ strip_tac \\ fs[Abbr`pc`]
+  \\ `s2.R 5w = s.R 5w`
+  by (
+    simp[Abbr`s2`]
+    \\ simp[ag32Theory.incPC_def, ag32Theory.dfn'LoadMEMByte_def,
+            ag32Theory.dfn'Normal_def, ag32Theory.norm_def,
+            ag32Theory.ri2word_def, ag32Theory.ALU_def]
+      \\ simp[APPLY_UPDATE_THM]
+      \\ simp[Abbr`s1`]
+      \\ simp[ag32Theory.dfn'JumpIfZero_def, ag32Theory.incPC_def,
+              ag32Theory.dfn'Normal_def, ag32Theory.norm_def,
+              ag32Theory.ri2word_def, ag32Theory.ALU_def] )
+  \\ `∀k. k < LENGTH ag32_ffi_copy_code ⇒
+      (get_mem_word s3.MEM (s.PC + n2w (4 * k)) =
+       Encode (EL k ag32_ffi_copy_code))`
+  by (
+    qx_gen_tac`k`
+    \\ strip_tac
+    \\ first_x_assum drule
+    \\ disch_then(SUBST1_TAC o SYM)
+    \\ simp[Abbr`s3`, ag32Theory.dfn'StoreMEMByte_def, ag32Theory.incPC_def, ag32Theory.ri2word_def]
+    \\ simp[get_mem_word_def, APPLY_UPDATE_THM]
+    \\ fs[EVAL``LENGTH ag32_ffi_copy_code``]
+    \\ Cases_on`s.R 5w` \\ Cases_on`s.PC` \\ fs[word_add_n2w]
+    \\ IF_CASES_TAC \\ fs[IN_DISJOINT, DISJ_EQ_IMP, PULL_EXISTS]
+    >- ( first_x_assum(qspec_then`0`mp_tac) \\ simp[DIV_LT_X]
+         \\ disch_then(qspec_then`4 * k + 3`mp_tac) \\ simp[])
+    \\ IF_CASES_TAC \\ fs[]
+    >- ( first_x_assum(qspec_then`0`mp_tac) \\ simp[DIV_LT_X]
+         \\ disch_then(qspec_then`4 * k + 2`mp_tac) \\ simp[])
+    \\ IF_CASES_TAC \\ fs[]
+    >- ( first_x_assum(qspec_then`0`mp_tac) \\ simp[DIV_LT_X]
+         \\ disch_then(qspec_then`4 * k + 1`mp_tac) \\ simp[])
+    \\ IF_CASES_TAC \\ fs[]
+    >- ( first_x_assum(qspec_then`0`mp_tac) \\ simp[DIV_LT_X]
+         \\ disch_then(qspec_then`4 * k + 0`mp_tac) \\ simp[]))
+  \\ first_assum(qspec_then`3`mp_tac)
+  \\ impl_tac >- EVAL_TAC
+  \\ simp[]
+  \\ disch_then kall_tac
+  \\ simp[ag32_targetProofTheory.Decode_Encode]
+  \\ simp[ag32_ffi_copy_code_def]
+  \\ simp[ag32Theory.Run_def]
+  \\ simp[Once EXISTS_NUM] \\ disj2_tac \\ simp[FUNPOW]
+  \\ qmatch_goalsub_abbrev_tac`Next s4`
+  \\ simp[ag32Theory.Next_def]
+  \\ qmatch_goalsub_abbrev_tac`pc + 2w`
+  \\ simp[GSYM get_mem_word_def]
+  \\ `s4.PC = s.PC + n2w (4 * 4)`
+  by ( simp[Abbr`s4`, dfn'Normal_PC])
+  \\ qpat_x_assum`Abbrev(pc = _)`mp_tac
+  \\ DEP_REWRITE_TAC[byte_aligned_imp]
+  \\ conj_tac
+  >- ( simp[] \\ irule byte_aligned_add \\ fs[] \\ EVAL_TAC )
+  \\ strip_tac \\ fs[Abbr`pc`]
+  \\ `s4.MEM = s3.MEM` by simp[Abbr`s4`, dfn'Normal_MEM]
+  \\ first_assum(qspec_then`4`mp_tac)
+  \\ impl_tac >- EVAL_TAC
+  \\ simp[]
+  \\ simp[ag32_targetProofTheory.Decode_Encode]
+  \\ simp[ag32_ffi_copy_code_def]
+  \\ disch_then kall_tac
+  \\ simp[ag32Theory.Run_def]
+  \\ simp[Once EXISTS_NUM] \\ disj2_tac \\ simp[FUNPOW]
+  \\ qmatch_goalsub_abbrev_tac`Next s5`
+  \\ simp[ag32Theory.Next_def]
+  \\ qmatch_goalsub_abbrev_tac`pc + 2w`
+  \\ simp[GSYM get_mem_word_def]
+  \\ `s5.PC = s.PC + n2w (4 * 5)`
+  by ( simp[Abbr`s5`, dfn'Normal_PC])
+  \\ qpat_x_assum`Abbrev(pc = _)`mp_tac
+  \\ DEP_REWRITE_TAC[byte_aligned_imp]
+  \\ conj_tac
+  >- ( simp[] \\ irule byte_aligned_add \\ fs[] \\ EVAL_TAC )
+  \\ strip_tac \\ fs[Abbr`pc`]
+  \\ `s5.MEM = s3.MEM` by simp[Abbr`s5`, dfn'Normal_MEM]
+  \\ first_assum(qspec_then`5`mp_tac)
+  \\ impl_tac >- EVAL_TAC
+  \\ simp[]
+  \\ simp[ag32_targetProofTheory.Decode_Encode]
+  \\ simp[ag32_ffi_copy_code_def]
+  \\ disch_then kall_tac
+  \\ simp[ag32Theory.Run_def]
+  \\ simp[Once EXISTS_NUM] \\ disj2_tac \\ simp[FUNPOW]
+  \\ qmatch_goalsub_abbrev_tac`Next s6`
+  \\ simp[ag32Theory.Next_def]
+  \\ qmatch_goalsub_abbrev_tac`pc + 2w`
+  \\ simp[GSYM get_mem_word_def]
+  \\ `s6.PC = s.PC + n2w (4 * 6)`
+  by ( simp[Abbr`s6`, dfn'Normal_PC])
+  \\ qpat_x_assum`Abbrev(pc = _)`mp_tac
+  \\ DEP_REWRITE_TAC[byte_aligned_imp]
+  \\ conj_tac
+  >- ( simp[] \\ irule byte_aligned_add \\ fs[] \\ EVAL_TAC )
+  \\ strip_tac \\ fs[Abbr`pc`]
+  \\ `s6.MEM = s3.MEM` by simp[Abbr`s6`, dfn'Normal_MEM]
+  \\ first_assum(qspec_then`6`mp_tac)
+  \\ impl_tac >- EVAL_TAC
+  \\ simp[]
+  \\ simp[ag32_targetProofTheory.Decode_Encode]
+  \\ simp[ag32_ffi_copy_code_def]
+  \\ disch_then kall_tac
+  \\ simp[ag32Theory.Run_def]
+  \\ qmatch_goalsub_abbrev_tac`_ = _ s7`
+  \\ last_x_assum(qspec_then`s7`mp_tac)
+  \\ impl_keep_tac
+  >-(
+    simp[Abbr`s7`, ag32Theory.dfn'JumpIfZero_def, ag32Theory.ri2word_def,ag32Theory.ALU_def]
+    \\ simp[Abbr`s6`, ag32Theory.dfn'Normal_def, ag32Theory.norm_def,
+            ag32Theory.ri2word_def,ag32Theory.ALU_def,ag32Theory.incPC_def,APPLY_UPDATE_THM]
+    \\ simp[Abbr`s5`, ag32Theory.dfn'Normal_def, ag32Theory.norm_def,
+            ag32Theory.ri2word_def,ag32Theory.ALU_def,ag32Theory.incPC_def,APPLY_UPDATE_THM]
+    \\ simp[Abbr`s4`, ag32Theory.dfn'Normal_def, ag32Theory.norm_def,
+            ag32Theory.ri2word_def,ag32Theory.ALU_def,ag32Theory.incPC_def,APPLY_UPDATE_THM]
+    \\ simp[Abbr`s3`, ag32Theory.dfn'StoreMEMByte_def,ag32Theory.incPC_def]
+    \\ simp[Abbr`s2`, ag32Theory.dfn'LoadMEMByte_def,ag32Theory.incPC_def,APPLY_UPDATE_THM]
+    \\ simp[Abbr`s1`, ag32Theory.dfn'JumpIfZero_def, ag32Theory.incPC_def, ag32Theory.ri2word_def,
+            ag32Theory.ALU_def]
+    \\ simp[ADD1,GSYM word_add_n2w])
+  \\ `s7.MEM = s3.MEM` by simp[Abbr`s7`, dfn'JumpIfZero_MEM]
+  \\ `s7.PC = s.PC`
+  by ( simp[Abbr`s7`, ag32Theory.dfn'JumpIfZero_def, ag32Theory.ri2word_def,ag32Theory.ALU_def])
+  \\ `s7.R 5w = s.R 5w + 1w`
+  by(
+    simp[Abbr`s7`, ag32Theory.dfn'JumpIfZero_def, ag32Theory.ri2word_def,ag32Theory.ALU_def]
+    \\ simp[Abbr`s6`, ag32Theory.dfn'Normal_def, ag32Theory.norm_def,
+            ag32Theory.ri2word_def,ag32Theory.ALU_def,ag32Theory.incPC_def,APPLY_UPDATE_THM]
+    \\ simp[Abbr`s5`, ag32Theory.dfn'Normal_def, ag32Theory.norm_def,
+            ag32Theory.ri2word_def,ag32Theory.ALU_def,ag32Theory.incPC_def,APPLY_UPDATE_THM]
+    \\ simp[Abbr`s4`, ag32Theory.dfn'Normal_def, ag32Theory.norm_def,
+            ag32Theory.ri2word_def,ag32Theory.ALU_def,ag32Theory.incPC_def,APPLY_UPDATE_THM]
+    \\ simp[Abbr`s3`, ag32Theory.dfn'StoreMEMByte_def,ag32Theory.incPC_def])
+  \\ disch_then match_mp_tac
+  \\ simp[]
+  \\ Cases_on`s.R 5w` \\ Cases_on`s7.R 1w` \\ fs[word_add_n2w]
+  \\ fs[ADD1,IN_DISJOINT,GSYM word_add_n2w,DISJ_EQ_IMP,PULL_EXISTS]
+  \\ rw[]
+  \\ `k + 1 <n' + 1`by simp[]
+  \\ first_x_assum drule
+  \\ fs[word_add_n2w]);
 
 val ag32_ffi_write_set_id_code_thm = Q.store_thm("ag32_ffi_write_set_id_code_thm",
   `(∀k. k < LENGTH ag32_ffi_write_set_id_code ⇒
@@ -191,50 +429,6 @@ val ag32_ffi_write_set_id_code_thm = Q.store_thm("ag32_ffi_write_set_id_code_thm
   \\ simp[ag32_targetProofTheory.Decode_Encode]
   \\ simp[ag32Theory.Run_def]
   \\ rw[Once EXISTS_NUM]);
-
-fun next_tac n =
-  let
-    val sn = mk_var("s"^(Int.toString n), ``:ag32_state``)
-  in
-    rw[Once EXISTS_NUM] \\ disj2_tac \\ rw[FUNPOW]
-    \\ qmatch_goalsub_abbrev_tac`Next ^sn`
-    \\ rw[ag32Theory.Next_def]
-    \\ qmatch_goalsub_abbrev_tac`pc + 2w`
-    \\ simp[GSYM get_mem_word_def]
-    \\ `^sn.PC = s.PC + n2w(4 * ^(numSyntax.term_of_int n))`
-    by ( simp[Abbr`^sn`,
-              dfn'Normal_PC,
-              dfn'LoadMEMByte_PC,
-              dfn'Shift_PC,
-              dfn'LoadConstant_PC] )
-    \\ `byte_aligned ^sn.PC`
-    by (
-      simp[]
-      \\ irule byte_aligned_add \\ simp[]
-      \\ EVAL_TAC )
-    \\ drule byte_aligned_imp
-    \\ simp[]
-    \\ disch_then kall_tac
-    \\ qpat_x_assum`Abbrev(pc = _)`kall_tac
-    \\ last_assum(qspec_then`^(numSyntax.term_of_int n)`mp_tac)
-    \\ impl_tac >- EVAL_TAC
-    \\ simp_tac(srw_ss())[ag32_ffi_write_check_conf_code_def,
-                          ag32_ffi_write_load_noff_code_def,
-                          ag32_ffi_write_check_lengths_code_def,
-                          ag32_ffi_write_write_header_code_def,
-                          ag32_ffi_write_num_written_code_def,
-                          ag32_ffi_write_copy_code_def]
-    \\ `^sn.MEM = s.MEM`
-    by simp[Abbr`^sn`,
-            dfn'Normal_MEM,
-            dfn'LoadMEMByte_MEM,
-            dfn'Shift_MEM,
-            dfn'LoadConstant_MEM]
-    \\ simp[]
-    \\ disch_then kall_tac
-    \\ simp[ag32_targetProofTheory.Decode_Encode]
-    \\ simp[ag32Theory.Run_def]
-  end
 
 val ag32_ffi_write_check_conf_code_thm = Q.store_thm("ag32_ffi_write_check_conf_code_thm",
   `(∀k. k < LENGTH ag32_ffi_write_check_conf_code ⇒
@@ -1133,229 +1327,6 @@ val ag32_ffi_write_num_written_code_thm = Q.store_thm("ag32_ffi_write_num_writte
   \\ simp[ag32Theory.Run_def]
   \\ simp[Once EXISTS_NUM]);
 
-val ag32_ffi_write_copy_code_thm = Q.store_thm("ag32_ffi_write_copy_code_thm",
-  `∀s.
-   (∀k. k < LENGTH ag32_ffi_write_copy_code ⇒
-        (get_mem_word s.MEM (s.PC + n2w (4 * k)) =
-         Encode (EL k ag32_ffi_write_copy_code)))
-   ∧ byte_aligned s.PC
-   ∧ w2n s.PC + 4 * LENGTH ag32_ffi_write_copy_code < dimword (:32)
-   ∧ w2n (s.R 5w) + w2n (s.R 1w) < dimword(:32)
-   ∧ DISJOINT { s.R 5w + n2w k | k | k < w2n (s.R 1w) }
-              { s.PC + n2w k | k | k DIV 4 < LENGTH ag32_ffi_write_copy_code }
-   ⇒
-   ∃k. (FUNPOW Next k s = ag32_ffi_write_copy s)`,
-  Induct_on`w2n(s.R 1w)` \\ rw[]
-  >- (
-    simp[Once ag32_ffi_write_copy_def]
-    \\ Cases_on`s.R 1w` \\ fs[] \\ rw[]
-    \\ qexists_tac`1` \\ rw[]
-    \\ rw[ag32Theory.Next_def]
-    \\ qmatch_goalsub_abbrev_tac`pc + 2w`
-    \\ simp[GSYM get_mem_word_def]
-    \\ last_assum(qspec_then`0`mp_tac)
-    \\ impl_tac >- EVAL_TAC
-    \\ simp_tac(srw_ss())[]
-    \\ pop_assum mp_tac
-    \\ DEP_REWRITE_TAC[byte_aligned_imp]
-    \\ conj_tac >- rw[]
-    \\ strip_tac \\ simp[Abbr`pc`]
-    \\ disch_then kall_tac
-    \\ simp[ag32_ffi_write_copy_code_def]
-    \\ simp[ag32_targetProofTheory.Decode_Encode]
-    \\ simp[ag32Theory.Run_def] )
-  \\ simp[Once ag32_ffi_write_copy_def]
-  \\ Cases_on`s.R 1w` \\ fs[]
-  \\ simp[Once EXISTS_NUM] \\ disj2_tac \\ simp[FUNPOW]
-  \\ simp[ag32Theory.Next_def]
-  \\ qmatch_goalsub_abbrev_tac`pc + 2w`
-  \\ simp[GSYM get_mem_word_def]
-  \\ qpat_x_assum`Abbrev(pc = _)`mp_tac
-  \\ DEP_REWRITE_TAC[byte_aligned_imp]
-  \\ conj_tac
-  >- ( simp[] \\ irule byte_aligned_add \\ fs[] \\ EVAL_TAC )
-  \\ strip_tac \\ fs[Abbr`pc`]
-  \\ first_assum(qspec_then`0`mp_tac)
-  \\ impl_tac >- EVAL_TAC
-  \\ simp[]
-  \\ simp[ag32_targetProofTheory.Decode_Encode]
-  \\ simp[ag32_ffi_write_copy_code_def]
-  \\ disch_then kall_tac
-  \\ simp[ag32Theory.Run_def]
-  \\ simp[Once EXISTS_NUM] \\ disj2_tac \\ simp[FUNPOW]
-  \\ qmatch_goalsub_abbrev_tac`Next s1`
-  \\ simp[ag32Theory.Next_def]
-  \\ qmatch_goalsub_abbrev_tac`pc + 2w`
-  \\ simp[GSYM get_mem_word_def]
-  \\ `s1.PC = s.PC + n2w (4 * 1)`
-  by ( simp[Abbr`s1`, ag32Theory.dfn'JumpIfZero_def, ag32Theory.ri2word_def,
-            ag32Theory.ALU_def,ag32Theory.incPC_def] )
-  \\ qpat_x_assum`Abbrev(pc = _)`mp_tac
-  \\ DEP_REWRITE_TAC[byte_aligned_imp]
-  \\ conj_tac
-  >- ( simp[] \\ irule byte_aligned_add \\ fs[] \\ EVAL_TAC )
-  \\ strip_tac \\ fs[Abbr`pc`]
-  \\ `s1.MEM = s.MEM` by simp[Abbr`s1`, dfn'JumpIfZero_MEM]
-  \\ first_assum(qspec_then`1`mp_tac)
-  \\ impl_tac >- EVAL_TAC
-  \\ simp[]
-  \\ simp[ag32_targetProofTheory.Decode_Encode]
-  \\ simp[ag32_ffi_write_copy_code_def]
-  \\ disch_then kall_tac
-  \\ simp[ag32Theory.Run_def]
-  \\ next_tac 2
-  \\ simp[Once EXISTS_NUM] \\ disj2_tac \\ simp[FUNPOW]
-  \\ qmatch_goalsub_abbrev_tac`Next s3`
-  \\ simp[ag32Theory.Next_def]
-  \\ qmatch_goalsub_abbrev_tac`pc + 2w`
-  \\ simp[GSYM get_mem_word_def]
-  \\ `s3.PC = s.PC + n2w (4 * 3)`
-  by ( simp[Abbr`s3`, ag32Theory.dfn'StoreMEMByte_def, ag32Theory.incPC_def] )
-  \\ qpat_x_assum`Abbrev(pc = _)`mp_tac
-  \\ DEP_REWRITE_TAC[byte_aligned_imp]
-  \\ conj_tac
-  >- ( simp[] \\ irule byte_aligned_add \\ fs[] \\ EVAL_TAC )
-  \\ strip_tac \\ fs[Abbr`pc`]
-  \\ `s2.R 5w = s.R 5w`
-  by (
-    simp[Abbr`s2`]
-    \\ simp[ag32Theory.incPC_def, ag32Theory.dfn'LoadMEMByte_def,
-            ag32Theory.dfn'Normal_def, ag32Theory.norm_def,
-            ag32Theory.ri2word_def, ag32Theory.ALU_def]
-      \\ simp[APPLY_UPDATE_THM]
-      \\ simp[Abbr`s1`]
-      \\ simp[ag32Theory.dfn'JumpIfZero_def, ag32Theory.incPC_def,
-              ag32Theory.dfn'Normal_def, ag32Theory.norm_def,
-              ag32Theory.ri2word_def, ag32Theory.ALU_def] )
-  \\ `∀k. k < LENGTH ag32_ffi_write_copy_code ⇒
-      (get_mem_word s3.MEM (s.PC + n2w (4 * k)) =
-       Encode (EL k ag32_ffi_write_copy_code))`
-  by (
-    qx_gen_tac`k`
-    \\ strip_tac
-    \\ first_x_assum drule
-    \\ disch_then(SUBST1_TAC o SYM)
-    \\ simp[Abbr`s3`, ag32Theory.dfn'StoreMEMByte_def, ag32Theory.incPC_def, ag32Theory.ri2word_def]
-    \\ simp[get_mem_word_def, APPLY_UPDATE_THM]
-    \\ fs[EVAL``LENGTH ag32_ffi_write_copy_code``]
-    \\ Cases_on`s.R 5w` \\ Cases_on`s.PC` \\ fs[word_add_n2w]
-    \\ IF_CASES_TAC \\ fs[IN_DISJOINT, DISJ_EQ_IMP, PULL_EXISTS]
-    >- ( first_x_assum(qspec_then`0`mp_tac) \\ simp[DIV_LT_X]
-         \\ disch_then(qspec_then`4 * k + 3`mp_tac) \\ simp[])
-    \\ IF_CASES_TAC \\ fs[]
-    >- ( first_x_assum(qspec_then`0`mp_tac) \\ simp[DIV_LT_X]
-         \\ disch_then(qspec_then`4 * k + 2`mp_tac) \\ simp[])
-    \\ IF_CASES_TAC \\ fs[]
-    >- ( first_x_assum(qspec_then`0`mp_tac) \\ simp[DIV_LT_X]
-         \\ disch_then(qspec_then`4 * k + 1`mp_tac) \\ simp[])
-    \\ IF_CASES_TAC \\ fs[]
-    >- ( first_x_assum(qspec_then`0`mp_tac) \\ simp[DIV_LT_X]
-         \\ disch_then(qspec_then`4 * k + 0`mp_tac) \\ simp[]))
-  \\ first_assum(qspec_then`3`mp_tac)
-  \\ impl_tac >- EVAL_TAC
-  \\ simp[]
-  \\ disch_then kall_tac
-  \\ simp[ag32_targetProofTheory.Decode_Encode]
-  \\ simp[ag32_ffi_write_copy_code_def]
-  \\ simp[ag32Theory.Run_def]
-  \\ simp[Once EXISTS_NUM] \\ disj2_tac \\ simp[FUNPOW]
-  \\ qmatch_goalsub_abbrev_tac`Next s4`
-  \\ simp[ag32Theory.Next_def]
-  \\ qmatch_goalsub_abbrev_tac`pc + 2w`
-  \\ simp[GSYM get_mem_word_def]
-  \\ `s4.PC = s.PC + n2w (4 * 4)`
-  by ( simp[Abbr`s4`, dfn'Normal_PC])
-  \\ qpat_x_assum`Abbrev(pc = _)`mp_tac
-  \\ DEP_REWRITE_TAC[byte_aligned_imp]
-  \\ conj_tac
-  >- ( simp[] \\ irule byte_aligned_add \\ fs[] \\ EVAL_TAC )
-  \\ strip_tac \\ fs[Abbr`pc`]
-  \\ `s4.MEM = s3.MEM` by simp[Abbr`s4`, dfn'Normal_MEM]
-  \\ first_assum(qspec_then`4`mp_tac)
-  \\ impl_tac >- EVAL_TAC
-  \\ simp[]
-  \\ simp[ag32_targetProofTheory.Decode_Encode]
-  \\ simp[ag32_ffi_write_copy_code_def]
-  \\ disch_then kall_tac
-  \\ simp[ag32Theory.Run_def]
-  \\ simp[Once EXISTS_NUM] \\ disj2_tac \\ simp[FUNPOW]
-  \\ qmatch_goalsub_abbrev_tac`Next s5`
-  \\ simp[ag32Theory.Next_def]
-  \\ qmatch_goalsub_abbrev_tac`pc + 2w`
-  \\ simp[GSYM get_mem_word_def]
-  \\ `s5.PC = s.PC + n2w (4 * 5)`
-  by ( simp[Abbr`s5`, dfn'Normal_PC])
-  \\ qpat_x_assum`Abbrev(pc = _)`mp_tac
-  \\ DEP_REWRITE_TAC[byte_aligned_imp]
-  \\ conj_tac
-  >- ( simp[] \\ irule byte_aligned_add \\ fs[] \\ EVAL_TAC )
-  \\ strip_tac \\ fs[Abbr`pc`]
-  \\ `s5.MEM = s3.MEM` by simp[Abbr`s5`, dfn'Normal_MEM]
-  \\ first_assum(qspec_then`5`mp_tac)
-  \\ impl_tac >- EVAL_TAC
-  \\ simp[]
-  \\ simp[ag32_targetProofTheory.Decode_Encode]
-  \\ simp[ag32_ffi_write_copy_code_def]
-  \\ disch_then kall_tac
-  \\ simp[ag32Theory.Run_def]
-  \\ simp[Once EXISTS_NUM] \\ disj2_tac \\ simp[FUNPOW]
-  \\ qmatch_goalsub_abbrev_tac`Next s6`
-  \\ simp[ag32Theory.Next_def]
-  \\ qmatch_goalsub_abbrev_tac`pc + 2w`
-  \\ simp[GSYM get_mem_word_def]
-  \\ `s6.PC = s.PC + n2w (4 * 6)`
-  by ( simp[Abbr`s6`, dfn'Normal_PC])
-  \\ qpat_x_assum`Abbrev(pc = _)`mp_tac
-  \\ DEP_REWRITE_TAC[byte_aligned_imp]
-  \\ conj_tac
-  >- ( simp[] \\ irule byte_aligned_add \\ fs[] \\ EVAL_TAC )
-  \\ strip_tac \\ fs[Abbr`pc`]
-  \\ `s6.MEM = s3.MEM` by simp[Abbr`s6`, dfn'Normal_MEM]
-  \\ first_assum(qspec_then`6`mp_tac)
-  \\ impl_tac >- EVAL_TAC
-  \\ simp[]
-  \\ simp[ag32_targetProofTheory.Decode_Encode]
-  \\ simp[ag32_ffi_write_copy_code_def]
-  \\ disch_then kall_tac
-  \\ simp[ag32Theory.Run_def]
-  \\ qmatch_goalsub_abbrev_tac`_ = _ s7`
-  \\ last_x_assum(qspec_then`s7`mp_tac)
-  \\ impl_keep_tac
-  >-(
-    simp[Abbr`s7`, ag32Theory.dfn'JumpIfZero_def, ag32Theory.ri2word_def,ag32Theory.ALU_def]
-    \\ simp[Abbr`s6`, ag32Theory.dfn'Normal_def, ag32Theory.norm_def,
-            ag32Theory.ri2word_def,ag32Theory.ALU_def,ag32Theory.incPC_def,APPLY_UPDATE_THM]
-    \\ simp[Abbr`s5`, ag32Theory.dfn'Normal_def, ag32Theory.norm_def,
-            ag32Theory.ri2word_def,ag32Theory.ALU_def,ag32Theory.incPC_def,APPLY_UPDATE_THM]
-    \\ simp[Abbr`s4`, ag32Theory.dfn'Normal_def, ag32Theory.norm_def,
-            ag32Theory.ri2word_def,ag32Theory.ALU_def,ag32Theory.incPC_def,APPLY_UPDATE_THM]
-    \\ simp[Abbr`s3`, ag32Theory.dfn'StoreMEMByte_def,ag32Theory.incPC_def]
-    \\ simp[Abbr`s2`, ag32Theory.dfn'LoadMEMByte_def,ag32Theory.incPC_def,APPLY_UPDATE_THM]
-    \\ simp[Abbr`s1`, ag32Theory.dfn'JumpIfZero_def, ag32Theory.incPC_def, ag32Theory.ri2word_def,
-            ag32Theory.ALU_def]
-    \\ simp[ADD1,GSYM word_add_n2w])
-  \\ `s7.MEM = s3.MEM` by simp[Abbr`s7`, dfn'JumpIfZero_MEM]
-  \\ `s7.PC = s.PC`
-  by ( simp[Abbr`s7`, ag32Theory.dfn'JumpIfZero_def, ag32Theory.ri2word_def,ag32Theory.ALU_def])
-  \\ `s7.R 5w = s.R 5w + 1w`
-  by(
-    simp[Abbr`s7`, ag32Theory.dfn'JumpIfZero_def, ag32Theory.ri2word_def,ag32Theory.ALU_def]
-    \\ simp[Abbr`s6`, ag32Theory.dfn'Normal_def, ag32Theory.norm_def,
-            ag32Theory.ri2word_def,ag32Theory.ALU_def,ag32Theory.incPC_def,APPLY_UPDATE_THM]
-    \\ simp[Abbr`s5`, ag32Theory.dfn'Normal_def, ag32Theory.norm_def,
-            ag32Theory.ri2word_def,ag32Theory.ALU_def,ag32Theory.incPC_def,APPLY_UPDATE_THM]
-    \\ simp[Abbr`s4`, ag32Theory.dfn'Normal_def, ag32Theory.norm_def,
-            ag32Theory.ri2word_def,ag32Theory.ALU_def,ag32Theory.incPC_def,APPLY_UPDATE_THM]
-    \\ simp[Abbr`s3`, ag32Theory.dfn'StoreMEMByte_def,ag32Theory.incPC_def])
-  \\ disch_then match_mp_tac
-  \\ simp[]
-  \\ Cases_on`s.R 5w` \\ Cases_on`s7.R 1w` \\ fs[word_add_n2w]
-  \\ fs[ADD1,IN_DISJOINT,GSYM word_add_n2w,DISJ_EQ_IMP,PULL_EXISTS]
-  \\ rw[]
-  \\ `k + 1 <n' + 1`by simp[]
-  \\ first_x_assum drule
-  \\ fs[word_add_n2w]);
-
 val ag32_ffi_write_code_thm = Q.store_thm("ag32_ffi_write_code_thm",
   `(∀k. k < LENGTH ag32_ffi_write_code ⇒
         (get_mem_word s.MEM (s.PC + n2w (4 * k)) =
@@ -1877,7 +1848,7 @@ val ag32_ffi_write_code_thm = Q.store_thm("ag32_ffi_write_code_thm",
   \\ strip_tac
   \\ qmatch_asmsub_abbrev_tac`_ = s6`
   \\ fs[]
-  \\ qspec_then`s6`mp_tac ag32_ffi_write_copy_code_thm
+  \\ qspec_then`s6`mp_tac ag32_ffi_copy_code_thm
   \\ `byte_aligned s6.PC`
   by (
     simp[Abbr`s6`]
@@ -1977,7 +1948,7 @@ val ag32_ffi_write_code_thm = Q.store_thm("ag32_ffi_write_code_thm",
       \\ EVAL_TAC \\ simp[GSYM word_add_n2w] )
     \\ simp[])
   \\ strip_tac
-  \\ qspec_then`s6`mp_tac ag32_ffi_write_copy_thm
+  \\ qspec_then`s6`mp_tac ag32_ffi_copy_thm
   \\ `s6.R 3w = s5.R 3w + 4w + n2w off`
   by (
     simp[Abbr`s6`, APPLY_UPDATE_THM]
@@ -2051,7 +2022,7 @@ val ag32_ffi_write_code_thm = Q.store_thm("ag32_ffi_write_code_thm",
     \\ full_simp_tac std_ss [GSYM ADD_ASSOC]
     \\ qmatch_asmsub_abbrev_tac`wcoff = _ + (_ + wcr)`
     \\ qpat_x_assum`∀k. k < LENGTH ag32_ffi_write_code ⇒ _`
-         (qspec_then`j + wcr DIV 4 + LENGTH ag32_ffi_write_copy_code + 2`mp_tac)
+         (qspec_then`j + wcr DIV 4 + LENGTH ag32_ffi_copy_code + 2`mp_tac)
     \\ impl_tac >- (
       simp[Abbr`wcr`]
       \\ qpat_x_assum`j <_`mp_tac
